

# Lecture Notes

Keshav Ramamurthy

February 11, 2026

## Contents

<b>1</b>	<b>2</b>
<b>2</b>	<b>2</b>
<b>3 Modular Practice</b>	<b>2</b>
3.1 (a) . . . . .	2
3.2 (b) . . . . .	2
3.3 (c) . . . . .	2
3.4 (d) . . . . .	2
3.5 (e) . . . . .	3
<b>4 Wilson's Theorem</b>	<b>3</b>

**1**

**2**

### 3 Modular Practice

#### 3.1 (a)

notice

$$9x + 5 \equiv 7 \pmod{13} \rightarrow 9x \equiv 7 - 5 \pmod{13} \rightarrow 9x \equiv 2 \pmod{13}$$

then, notice that  $9 \cdot 3 \equiv 27 \equiv 1 \pmod{13}$ , so multiplying by 3 on both sides yields

$$9 \cdot 3 \cdot x \equiv 2 \cdot 3 \pmod{13} \rightarrow \boxed{x \equiv 6 \pmod{13}}$$

#### 3.2 (b)

notice

$$3x + 12 \equiv 4 \pmod{21} \rightarrow 3x \equiv -8$$

then, we have that

$$3x \equiv 13 \pmod{21}$$

then, since the lhs is divisible by 3, notice that since the rhs is  $13 \pmod{21}$ , that this is equivalent to

$$21w + 13 \equiv 1 \pmod{3}$$

because the rhs and lhs have different parities mod 3, there are no solutions  $\square$

#### 3.3 (c)

let's write the systems first

$$5x + 4y \equiv 0 \pmod{7}$$

$$2x + y \equiv 4 \pmod{7}$$

notice that  $y \equiv 4 - 2x \pmod{7}$ , and that thus we can substitute that into the top equation yielding

$$5x + 4(4 - 2x) \equiv 0 \pmod{7} \rightarrow -3x + 16 \equiv 0 \pmod{7} \rightarrow 3x \equiv 16 \pmod{7} \rightarrow 3 \cdot 5 \cdot x \equiv 16 \cdot 5 \pmod{7}$$

This reduces to  $x \equiv 3 \pmod{7}$  yielding  $y \equiv 4 - 2x \equiv 5 \pmod{7}$

#### 3.4 (d)

Notice

$$(13)^{2023} = (12 + 1)^{2023} \equiv (0 + 1)^{2023} \equiv 1^{2023} \equiv 1 \pmod{7}$$

### 3.5 (e)

By Fermat's little theorem, since 11 is prime, we have that

$$7^{11-1} = 7^{10} \equiv 1 \pmod{11}$$

Then,

$$7^{62} \equiv 7^{60} 7^2 \equiv (7^{10})^6 7^2 \equiv 7^2 \equiv 5 \pmod{11}$$

## 4 Wilson's Theorem

Let us first show that if  $p$  is prime, that this holds. Then, we will prove the other direction. We'll first show every residue  $r \pmod{p}$  except 0 has an inverse  $\pmod{p}$ . Notice if  $r$  has an inverse

$$\exists r^{-1} \in (\mathbb{Z}/p\mathbb{Z})^\times \mid rr^{-1} \equiv 1 \pmod{p}$$

We know that every number  $r \in (\mathbb{Z}/p\mathbb{Z})^\times$  has an inverse by Bezout's identity, since  $\gcd(r, p) = 1$ . We claim that that the pairs

$$(1, 1), (p-1, p-1), (r_1, r_1^{-1}), (r_2, r_2^{-1}), (r_3, r_3^{-1}), \dots, (r_{\frac{p-3}{2}}, r_{\frac{p-3}{2}}^{-1})$$

contain all the numbers in  $(\mathbb{Z}/p\mathbb{Z})^\times$  exactly once (except for 1 and  $p-1$ )

Notice for any residue  $r$ , that its inverse must be unique, as if  $r$  had two inverses  $i_1^{-1}, i_2^{-1}$ , then we'd have that

$$ri_1^{-1} \equiv ri_2^{-1} \equiv 1 \rightarrow r(i_1^{-1} - i_2^{-1}) \equiv 0 \rightarrow i_1^{-1} = i_2^{-1}$$

which is false my contradiction. However, its inverse may not be distinct from  $r$ , so let's examine the case that  $r \cdot r \equiv 1 \pmod{p}$

Notice this turns into

$$r^2 - 1 \equiv 0 \pmod{p} \rightarrow r \equiv 1, -1 \pmod{p}$$

So, two of our pairs are  $(1, 1)$  and  $(p-1, p-1)$ , but the rest are distinct, which then contain  $(\mathbb{Z}/p\mathbb{Z})^\times$

Thus, if every residue  $r$  must have a unique inverse, and an inverse exists for every residue, they have to pair up and contain all the numbers in  $(\mathbb{Z}/p\mathbb{Z})^\times$ . Now, notice that

$$(p-1)! \equiv \prod_{i=1}^{p-1} i \equiv \prod_{i=1}^{\frac{p-3}{2}} (r_i r_i^{-1}) \cdot 1 \cdot (p-1) \equiv (1)^{\frac{p-3}{2}} \cdot 1 \cdot -1 \equiv -1 \pmod{p} \quad \square$$

Notice that we can prove it forward pretty easily, the statement: If  $(p-1)! \equiv 1 \pmod{p}$ , then  $p$  is prime.

We can solve this with proof by contraposition. Notice that  $\neg Q$  is simply that  $p$  is not prime, and  $\neg P$  is

$$(p-1)! \not\equiv -1 \pmod{p}$$

If  $\neg Q$ , that  $\exists d \{d \in (1, 2, 3, \dots, P-1)\} (d \mid P)$

Now notice that if  $d \mid P$ ,  $d \nmid P-1$ , as  $d \neq 1$ . Thus,  $d \mid (p-1)!$ , yet the RHS can not be equivalent to -1 again because  $d \nmid P-1$ , so we are done  $\square$